CollapsingTowers/TwoLevelRec/Utils/List.lean
@@ -1,0 +1,79 @@
+import Mathlib.Data.Nat.Basic
+
+@[simp]
+def getr {α : Type} (x : ℕ) (l : List α) : Option α :=
+  match l with
+  | [] => none
+  | head :: tails => if tails.length == x then some head else getr x tails
+
+lemma getr_exists_iff_index_lt_length : ∀ {α : Type} (l : List α) i, i < l.length ↔ ∃ a, getr i l = some a :=
+  by
+  intro _ l i; constructor
+  . intro H; induction l
+    case nil => nomatch H
+    case cons tails IH =>
+      simp; by_cases HEq : tails.length = i
+      . simp [HEq]
+      . simp [if_neg HEq]; apply IH; simp at H; omega
+  . intro H; induction l
+    case nil => nomatch H
+    case cons tails IH =>
+      simp at H; by_cases HEq : tails.length = i
+      . subst HEq; simp
+      . simp [if_neg HEq] at H; simp
+        have _ := IH H; omega
+
+@[simp]
+def binds {α : Type} (x : ℕ) (a : α) (l : List α) :=
+  getr x l = some a
+
+lemma binds.extend : ∀ {α : Type} Γ Δ x (a : α), binds x a Γ → binds x a (Δ ++ Γ) :=
+  by
+  intros _ Γ Δ x a Hbinds
+  induction Δ with
+  | nil => apply Hbinds
+  | cons head tails IHtails =>
+    simp
+    by_cases Hx : tails.length + Γ.length = x
+    . have Hx : x < Γ.length := by rw [getr_exists_iff_index_lt_length]; exists a
+      omega
+    . rw [if_neg Hx]; apply IHtails
+
+lemma binds.extendr : ∀ {α : Type} Γ Δ x (a : α), binds x a Γ → binds (x + Δ.length) a (Γ ++ Δ) :=
+  by
+  intros _ Γ Δ x a
+  induction Γ with
+  | nil => simp
+  | cons head tails IHtails =>
+    simp
+    by_cases HEq : tails.length = x
+    . repeat rw [if_pos HEq]; simp
+    . repeat rw [if_neg HEq]
+      apply IHtails
+
+lemma binds.shrink : ∀ {α : Type} Γ Δ x (a : α), x < Γ.length → binds x a (Δ ++ Γ) → binds x a Γ :=
+  by
+  intros _ Γ Δ x a HLt
+  induction Δ with
+  | nil => simp
+  | cons head tails IHtails =>
+    intro Hbinds; apply IHtails
+    simp at *
+    have HNe : tails.length + Γ.length ≠ x := by omega
+    rw [if_neg HNe] at Hbinds
+    apply Hbinds
+
+lemma binds.shrinkr : ∀ {α : Type} Γ Δ x (a : α), binds (x + Δ.length) a (Γ ++ Δ) → binds x a Γ :=
+  by
+  intros _ Γ Δ x a
+  induction Γ with
+  | nil =>
+    simp; intro Hgetr
+    have : x + Δ.length < Δ.length := by rw [getr_exists_iff_index_lt_length]; exists a
+    omega
+  | cons head tails IHtails =>
+    simp
+    by_cases HEq : tails.length = x
+    . repeat rw [if_pos HEq]; simp
+    . repeat rw [if_neg HEq]
+      apply IHtails
